src/Ex/Mesi/MesiInvExcl.v
@@ -1,0 +1,97 @@
+Require Import Bool List String Peano_dec Lia.
+Require Import Common FMap IndexSupport HVector Syntax Topology Semantics SemFacts StepM.
+Require Import Invariant TrsInv Simulation Serial SerialFacts.
+Require Import RqRsLang RqRsInvMsg RqRsCorrect.
+
+Require Import Ex.Spec Ex.SpecInds Ex.Template.
+Require Import Ex.Mesi Ex.Mesi.Mesi Ex.Mesi.MesiTopo.
+
+Require Import Ex.Mesi.MesiInv.
+
+Set Implicit Arguments.
+
+Import PropMonadNotations.
+Import CaseNotations.
+
+Local Open Scope list.
+Local Open Scope hvec.
+Local Open Scope fmap.
+
+Existing Instance Mesi.ImplOStateIfc.
+
+Definition NoDirE (oss: OStates) :=
+  forall oidx, ost <+- oss@[oidx]; ost#[dir].(dir_st) <> mesiE.
+
+Definition ObjsInvalid (eidx: IdxT) (oss: OStates) (msgs: MessagePool Msg) :=
+  forall oidx,
+    oidx <> eidx ->
+    ost <+- oss@[oidx]; ObjInvalid oidx ost msgs.
+
+Definition InvObjExcl0 (oidx: IdxT) (ost: OState) (oss: OStates)
+           (msgs: MessagePool Msg) :=
+  ObjExcl0 oidx ost msgs ->
+  ObjsInvalid oidx oss msgs /\ NoCohMsgs oidx msgs /\ NoDirE oss.
+
+Definition InvExcl (st: MState): Prop :=
+  forall eidx,
+    eost <+- (bst_oss st)@[eidx];
+      InvObjExcl0 eidx eost (bst_oss st) (bst_msgs st).
+
+Section Facts.
+
+  Lemma InvExcl_excl_invalid:
+    forall st (He: InvExcl st) msgs eidx eost,
+      bst_msgs st = msgs ->
+      (bst_oss st)@[eidx] = Some eost ->
+      NoRsI eidx msgs ->
+      mesiE <= eost#[status] ->
+      forall oidx ost,
+        oidx <> eidx ->
+        (bst_oss st)@[oidx] = Some ost ->
+        ObjInvalid oidx ost msgs.
+  Proof.
+    intros; subst.
+    specialize (He eidx).
+    disc_rule_conds_ex.
+    red in He.
+    unfold ObjExcl0 in He; simpl in He.
+    specialize (He (conj H2 H1)); dest.
+    specialize (H _ H3).
+    rewrite H4 in H; auto.
+  Qed.
+
+  Corollary InvExcl_excl_invalid_status:
+    forall st (He: InvExcl st) eidx eost,
+      (bst_oss st)@[eidx] = Some eost ->
+      NoRsI eidx (bst_msgs st) ->
+      mesiE <= eost#[status] ->
+      forall oidx ost,
+        oidx <> eidx ->
+        (bst_oss st)@[oidx] = Some ost ->
+        NoRsI oidx (bst_msgs st) ->
+        ost#[status] = mesiI.
+  Proof.
+    intros.
+    eapply InvExcl_excl_invalid in H1; eauto.
+    destruct H1.
+    - apply H1.
+    - exfalso; eapply NoRsI_MsgExistsSig_InvRs_false; eauto.
+  Qed.
+  
+End Facts.
+
+Section InvExcl.
+  Variable (tr: tree).
+  Hypothesis (Htr: tr <> Node nil).
+
+  Let topo: DTree := fst (tree2Topo tr 0).
+  Let cifc: CIfc := snd (tree2Topo tr 0).
+  Let impl: System := impl Htr.
+
+  Lemma mesi_InvExcl_ok:
+    Invariant.InvReachable impl step_m InvExcl.
+  Proof.
+  Admitted.
+
+End InvExcl.
+
